WebAssembly/Wasm_Axioms.thy
@@ -15,6 +15,20 @@ lemma mem_grow_size:
   unfolding mem_grow_def old_mem_size_def mem_append_def bytes_replicate_def
   by (auto simp add: Ki64_def Let_def split: prod.splits if_splits)
 
+lemma mem_grow_max1:
+  assumes "mem_grow m n = Some m'"
+  shows "mem_max m = mem_max m'"
+  using assms Abs_mem_inverse
+  unfolding mem_grow_def mem_max_def mem_append_def 
+  by (auto simp add: Ki64_def Let_def split: prod.splits if_splits)
+
+lemma mem_grow_max2:
+  assumes "mem_grow m n = Some m'"
+  shows "pred_option ((\<le>) (mem_size m')) (mem_max m')"
+  using assms Abs_mem_inverse
+  unfolding mem_grow_def mem_max_def mem_append_def
+  by (auto simp add: assms mem_grow_size Let_def split: prod.splits if_splits)
+
 lemma mem_grow_length:
   assumes "mem_grow m n = Some m'"
   shows "(mem_length m + (n * Ki64)) = mem_length m'"
@@ -63,6 +77,13 @@ lemma store_size:
   unfolding store_def write_bytes_def bytes_takefill_def
   by (cases "n + off + l \<le> mem_length m") (auto simp add: old_mem_size_def split: prod.splits)
 
+lemma store_max:
+  assumes "(store m n off v l = Some m')"
+  shows "mem_max m = mem_max m'"
+  using assms Abs_mem_inverse
+  unfolding store_def mem_max.rep_eq write_bytes_def
+  by (auto split: if_splits prod.splits)
+
 lemma store_length:
   assumes "(store m n off v l = Some m')"
   shows "mem_length m = mem_length m'"
@@ -80,6 +101,13 @@ lemma store_packed_size:
   assumes "(store_packed m n off v l = Some m')"
   shows "mem_size m = mem_size m'"
   using assms store_size
+  unfolding store_packed_def
+  by simp
+
+lemma store_packed_max:
+  assumes "(store_packed m n off v l = Some m')"
+  shows "mem_max m = mem_max m'"
+  using assms store_max
   unfolding store_packed_def
   by simp
 
